Weaken pred1 a bit to not reduce "new" redexes

pcuic/theories/PCUICRho.v
@@ -6,7 +6,8 @@ From Coq Require Import Bool List Utf8
 From MetaCoq.Template Require Import config utils.
 From MetaCoq.PCUIC Require Import PCUICAst PCUICAstUtils PCUICSize
      PCUICLiftSubst PCUICSigmaCalculus PCUICUnivSubst PCUICTyping PCUICReduction PCUICSubstitution
-     PCUICReflect PCUICClosed PCUICParallelReduction.
+     PCUICReflect PCUICClosed PCUICParallelReduction
+     PCUICParallelReductionConfluence.
 
 (* Type-valued relations. *)
 Require Import CRelationClasses.
@@ -566,5 +567,545 @@ Section Rho.
     simpl. eapply symmetry, decompose_app_inv in eqapp.
     subst x. destruct t; simpl in d => //.
   Qed.
+
+  Lemma rho_rename Γ Δ r t :
+    renaming Γ Δ r ->
+    rename r (rho Γ t) = rho Δ (rename r t).
+  Proof.
+  Admitted.
+
+
+  Section rho_ctx.
+    Context (Δ : context).
+    Fixpoint rho_ctx_over Γ :=
+      match Γ with
+      | [] => []
+      | {| decl_name := na; decl_body := None; decl_type := T |} :: Γ =>
+        let Γ' := rho_ctx_over Γ in
+        vass na (rho (Δ ,,, Γ') T) :: Γ'
+      | {| decl_name := na; decl_body := Some b; decl_type := T |} :: Γ =>
+        let Γ' := rho_ctx_over Γ in
+        vdef na (rho (Δ ,,, Γ') b) (rho (Δ ,,, Γ') T) :: Γ'
+      end.
+  End rho_ctx.
+
+  Definition rho_ctx Γ := (rho_ctx_over [] Γ).
+
+  Lemma rho_ctx_over_length Δ Γ : #|rho_ctx_over Δ Γ| = #|Γ|.
+  Proof.
+    induction Γ; simpl; auto. destruct a. destruct decl_body; simpl; auto with arith.
+  Qed.
+
+  Lemma rho_ctx_over_app Γ' Γ Δ :
+    rho_ctx_over Γ' (Γ ,,, Δ) =
+    rho_ctx_over Γ' Γ ,,, rho_ctx_over (Γ' ,,, rho_ctx_over Γ' Γ) Δ.
+  Proof.
+    induction Δ; simpl; auto.
+    destruct a as [na [b|] ty]. simpl. f_equal; auto.
+    now rewrite IHΔ app_context_assoc.
+    now rewrite IHΔ app_context_assoc.
+  Qed.
+
+  Lemma rho_ctx_app Γ Δ : rho_ctx (Γ ,,, Δ) = rho_ctx Γ ,,, rho_ctx_over (rho_ctx Γ) Δ.
+  Proof.
+    induction Δ; simpl; auto.
+    destruct a as [na [b|] ty]. simpl. f_equal.
+    rewrite app_context_nil_l. now rewrite IHΔ. auto.
+    rewrite app_context_nil_l. now rewrite IHΔ.
+  Qed.
+
+  Context {cf:checker_flags} (wfΣ : wf Σ).
+  Lemma rho_triangle_All_All2_ind:
+    ∀ (Γ : context) (brs : list (nat * term)),
+    pred1_ctx Σ Γ (rho_ctx Γ) →
+    All (λ x : nat * term, pred1_ctx Σ Γ (rho_ctx Γ) → pred1 Σ Γ (rho_ctx Γ) (snd x) (rho (rho_ctx Γ) (snd x)))
+        brs →
+    All2 (on_Trel_eq (pred1 Σ Γ (rho_ctx Γ)) snd fst) brs
+         (map (λ x : nat * term, (fst x, rho (rho_ctx Γ) (snd x))) brs).
+  Proof.
+    intros. rewrite - {1}(map_id brs). eapply All2_map, All_All2; eauto.
+  Qed.
+
+  Lemma rho_triangle_All_All2_ind_noeq:
+    ∀ (Γ Γ' : context) (brs0 brs1 : list (nat * term)),
+      pred1_ctx Σ Γ Γ' →
+      All2 (on_Trel_eq (λ x y : term, (pred1 Σ Γ Γ' x y * pred1 Σ Γ' (rho_ctx Γ) y (rho (rho_ctx Γ) x))%type) snd
+                       fst) brs0 brs1 ->
+      All2 (on_Trel (pred1 Σ Γ' (rho_ctx Γ)) snd) brs1 (map (λ x : nat * term, (fst x, rho (rho_ctx Γ) (snd x))) brs0).
+  Proof.
+    intros. rewrite - {1}(map_id brs1). eapply All2_map, All2_sym, All2_impl; pcuic.
+  Qed.
+
+
+  Lemma triangle Γ Δ t u :
+  let Pctx :=
+      fun (Γ Δ : context) => pred1_ctx Σ Δ (rho_ctx Γ) in
+  pred1 Σ Γ Δ t u -> pred1 Σ Δ (rho_ctx Γ) u (rho (rho_ctx Γ) t).
+  Proof with solve_discr.
+  intros Pctx H. revert Γ Δ t u H.
+  refine (pred1_ind_all_ctx Σ _ Pctx _ _ _ _ _ _ _ _ _ _ _ _ _ _ _ _ _ _ _ _ _ _);
+    subst Pctx; intros *.
+  all:try intros **; rename_all_hyps;
+    try solve [specialize (forall_Γ _ X3); eauto]; eauto;
+      try solve [simpl; econstructor; simpl; eauto].
+
+  simpl.
+  - induction X0; simpl; depelim predΓ'; constructor; rewrite ?app_context_nil_l; eauto.
+    all:simpl NoConfusion in *; noconf H; noconf H0; auto.
+
+  - simpl.
+    rewrite (rho_app_lambda _ _ _ _ _ []).
+    eapply (substitution0_pred1); simpl in *. eauto. eauto.
+    rewrite app_context_nil_l in X0.
+    eapply X0.
+
+  - simp rho.
+    eapply (substitution0_let_pred1); simpl in *. eauto. eauto.
+    rewrite app_context_nil_l in X4.
+    eapply X4.
+
+  - simp rho.
+    destruct nth_error eqn:Heq. simpl in X0.
+    pose proof Heq. apply nth_error_Some_length in Heq.
+    destruct c as [na [?|] ?]; noconf heq_option_map.
+    simpl in X0.
+    eapply (f_equal (option_map decl_body)) in H.
+    eapply nth_error_pred1_ctx_l in H; eauto.
+    destruct H. intuition. rewrite a. simp rho.
+    rewrite -{1}(firstn_skipn (S i) Γ').
+    rewrite -{1}(firstn_skipn (S i) (rho_ctx Γ)).
+    pose proof (All2_local_env_length X0).
+    assert (S i = #|firstn (S i) Γ'|).
+    rewrite !firstn_length_le; try lia.
+    assert (S i = #|firstn (S i) (rho_ctx Γ)|).
+    rewrite !firstn_length_le; try lia.
+    rewrite {5}H0 {6}H1.
+    eapply weakening_pred1_pred1; eauto.
+    eapply All2_local_env_over_firstn_skipn. auto.
+    noconf heq_option_map.
+
+  - simp rho. simpl in *.
+    destruct option_map eqn:Heq.
+    destruct o. constructor; auto.
+    constructor. auto.
+    constructor. auto.
+
+  - simpl in X0. cbn.
+    rewrite rho_app_case.
+    rewrite decompose_app_mkApps; auto.
+    change eq_inductive with (@eqb inductive _).
+    destruct (eqb_spec ind ind); try discriminate.
+    2:{ congruence. }
+    unfold iota_red. eapply pred_mkApps; eauto.
+    eapply pred_snd_nth. red in X2.
+    now eapply rho_triangle_All_All2_ind_noeq. auto.
+    eapply All2_skipn. eapply All2_sym.
+    rewrite - {1} (map_id args1). eapply All2_map, All2_impl; eauto. simpl. intuition.
+
+  - (* Fix reduction *)
+    unfold PCUICTyping.unfold_fix in heq_unfold_fix |- *.
+    rewrite rho_app_fix.
+    destruct nth_error eqn:Heq; noconf heq_unfold_fix.
+    destruct isLambda; try discriminate. noconf heq_unfold_fix.
+    eapply All2_nth_error_Some_right in Heq; eauto.
+    destruct Heq as [t' [Hnth Hrel]].
+    destruct Hrel as [[Hty Hrhoty] [[Hreleq0 Hreleq1] Heq]].
+    rewrite Hnth. simpl.
+    destruct args0. depelim X4. unfold is_constructor in heq_is_constructor.
+    rewrite nth_error_nil in heq_is_constructor => //.
+    pose proof Hnth.
+    eapply All2_nth_error_Some in H; eauto.
+    destruct H as [fn' [Hnth' [? ?]]].
+    destruct t', d.
+    simpl in * |-. noconf Heq. destruct o, p as [[ol ol'] or].
+    simpl in * |-. noconf or.
+    revert X4. generalize (t :: args0). clear t args0. intros args0 Hargs.
+    simpl.
+    move: heq_is_constructor.
+    unfold is_constructor.
+    case enth: nth_error => [a|] /= //.
+    eapply (All2_nth_error_Some_right _ _ Hargs) in enth as [t' [-> [redt' redat']]].
+    simpl in redt'. simpl.
+    move/(isConstruct_app_pred1 redat') => ->.
+    move ->.
+    eapply pred_mkApps.
+    rewrite rho_ctx_app in Hreleq1.
+    rewrite !subst_inst. simpl_pred.
+    rewrite /rho_fix_context -fold_fix_context_rho_ctx.
+    eapply strong_substitutivity; eauto.
+    apply ctxmap_fix_subst.
+    rewrite -rho_fix_subst -{1}fix_context_map_fix.
+    apply ctxmap_fix_subst.
+    rewrite -rho_fix_subst.
+    eapply All2_prop2_eq_split in X3.
+    apply pred_subst_rho_fix; intuition auto.
+    eapply All2_sym, All2_map_left, All2_impl; eauto. simpl. unfold on_Trel in *.
+    intuition eauto.
+
+    simpl.
+    (* Impossible: the body of a fix has to be a lambda *)
+    destruct dbody0; try discriminate.
+    clear -wfΣ Hreleq1 e. depelim Hreleq1. solve_discr.
+    rewrite rho_ctx_app in H. rewrite /rho_fix_context in e.
+    rewrite -fold_fix_context_rho_ctx in e. rewrite H in e.
+    discriminate. depelim i.
+
+  - (* Case-CoFix reduction *)
+    simpl. destruct ip.
+    rewrite decompose_app_mkApps; auto.
+    rewrite rho_mkApps // decompose_app_mkApps; auto.
+    simpl. unfold unfold_cofix in heq_unfold_cofix |- *.
+    rewrite nth_error_map.
+    destruct nth_error eqn:Heq; noconf heq_unfold_cofix. simpl.
+    eapply All2_prop2_eq_split in X3. intuition.
+    eapply All2_nth_error_Some_right in Heq; eauto.
+    destruct Heq as [t' [Ht' Hrel]]. rewrite Ht'. simpl.
+    eapply pred_case. eauto. eapply pred_mkApps.
+    red in Hrel. destruct Hrel.
+    rewrite rho_ctx_app in p2.
+    rewrite - fold_fix_context_rho_ctx.
+    set (rhoΓ := rho_ctx Γ ,,, rho_ctx_over (rho_ctx Γ) (fix_context mfix0)) in *.
+    rewrite !subst_inst. eapply simpl_pred; try now sigma.
+    eapply strong_substitutivity. eauto. apply ctxmap_cofix_subst.
+    unfold rhoΓ.
+    rewrite -{1}fix_context_map_fix.
+    now eapply ctxmap_cofix_subst.
+    now eapply pred_subst_rho_cofix; auto.
+    eapply All2_sym, All2_map_left, All2_impl; eauto. simpl. intuition eauto.
+    eapply All2_sym, All2_map_left, All2_impl; eauto. simpl. unfold on_Trel in *.
+    intuition eauto.
+
+  - (* Proj-Cofix reduction *)
+    simpl.
+    destruct p as [[ind pars] arg].
+    rewrite decompose_app_mkApps. auto.
+    rewrite rho_mkApps // decompose_app_mkApps // /=.
+    unfold unfold_cofix in heq_unfold_cofix |- *.
+    destruct nth_error eqn:Heq; noconf heq_unfold_cofix.
+    eapply All2_nth_error_Some_right in Heq; eauto.
+    destruct Heq as [t' [Hnth Hrel]]. destruct Hrel as [[Hty Hrhoty] [[Hreleq0 Hreleq1] Heq]].
+    unfold map_fix. rewrite nth_error_map Hnth /=.
+    econstructor. eapply pred_mkApps; eauto.
+    rewrite - fold_fix_context_rho_ctx.
+    rewrite rho_ctx_app in Hreleq1.
+    eapply substitution_pred1; eauto.
+    rewrite rho_cofix_subst.
+    { eapply wf_rho_cofix_subst; eauto.
+      now eapply All2_length in X3. }
+    eapply All2_sym, All2_map_left, All2_impl; eauto; simpl; intuition eauto.
+
+  - simpl. simpl in X0. red in H. rewrite H heq_cst_body. now eapply pred1_refl_gen.
+
+  - simpl in *. destruct (lookup_env Σ c) eqn:Heq; pcuic. destruct g; pcuic.
+    destruct cst_body eqn:Heq'; pcuic.
+    
+  - simpl in *. rewrite decompose_app_mkApps; auto.
+    rewrite rho_mkApps; auto.
+    rewrite decompose_app_mkApps; auto.
+    simpl. rewrite nth_error_map.
+    eapply All2_nth_error_Some_right in heq_nth_error as [t' [? ?]]; eauto.
+    simpl in y. rewrite e. simpl.
+    change eq_inductive with (@eqb inductive _).
+    destruct (eqb_spec i i) => //.
+
+  - simpl. eapply pred_abs; auto. unfold snoc in *. simpl in X2.
+    rewrite app_context_nil_l in X2. apply X2.
+
+  - case le': (isFix_app (tApp M0 N0)).
+    + (* Fix at head *)
+      rewrite rho_app_unfold /rho_app.
+      case e: decompose_app => [hd args].
+      eapply decompose_app_inv' in e as [Hhd Heq].
+      destruct args using rev_ind. simpl in Heq. rewrite -Heq in Hhd. discriminate.
+      clear IHargs. rewrite -mkApps_nested in Heq. noconf Heq.
+      apply isFix_app_inv in le' => //.
+      destruct hd; try discriminate.
+      move: X0.
+      rewrite -rho_fix_unfold.
+      destruct (rho_fix_elim (rho_ctx Γ) mfix idx args).
+      move/andP: i => [isl isc].
+      destruct (rho_fix_elim (rho_ctx Γ) mfix idx (args ++ [N0])).
+      * (* Both reduce *)
+        rewrite e in e0. noconf e0.
+        rewrite map_app in i.
+        move/andP: i => [isl' isc'].
+        rewrite (is_constructor_app_ge (rarg d) _ _) in isc' => //.
+        rewrite map_app - !mkApps_nested.
+        move=> redo. eapply (pred_mkApps _ _ _ _ _ [N1]) => //.
+        repeat constructor; auto.
+      * (* Shorter appliction reduces, longer one doesn't: impossible *)
+        elimtype False.
+        rewrite e in y. cbn in y. rewrite isl in y.
+        destruct y; auto.
+        rewrite map_app (is_constructor_app_ge (rarg d) _ _) in H => //.
+      * (* Shorter application does not reduce *)
+        destruct (rho_fix_elim (rho_ctx Γ) mfix idx (args ++ [N0])).
+        ** (* Longer application reduces *)
+          rewrite e in y.
+          rewrite map_app in i.
+          move/andP: i => [isl' isc'].
+          simpl in y. rewrite isl' in y.
+          assert (~~ is_constructor (rarg d) (map (rho (rho_ctx Γ)) args) /\ rarg d = #|args|) as [isc rargl].
+          { destruct y => //. split; auto.
+            move: isc' H; rewrite /is_constructor.
+            rewrite !nth_error_map.
+            destruct (Nat.leb_spec (S (rarg d)) #|args|).
+            rewrite nth_error_app_lt ?map_length //.
+            rewrite !nth_error_map. move => ->. discriminate.
+            rewrite nth_error_app_ge ?map_length //. lia.
+            simpl.
+            case e': nth_error => [arg'|]. simpl.
+            move => isC _. eapply nth_error_Some_length in e'. simpl in e'. lia.
+            discriminate. }
+          simpl.
+          case: (pred1_mkApps_tFix_inv _ _ _ _ _ _ _ X).
+          { move=> [mfix1 [args1 [[HM1 Hmfix] Hargs]]].
+            move: HM1 X => -> X.
+            rewrite [tApp _ _](mkApps_nested _ _ [N1]).
+            move/pred1_mkApps_tFix_refl_inv => [redo redargs].
+            rewrite map_app.
+            eapply pred_fix; eauto with pcuic.
+            eapply pred1_rho_fix_context_2; auto with pcuic.
+            red in redo. solve_all.
+            unfold on_Trel in *. intuition auto. now noconf b0.
+            now noconf b0.
+            unfold unfold_fix. rewrite nth_error_map e /=.
+            rewrite /rho_fix_context in isl'. rewrite isl'.
+            rewrite map_fix_subst /= //.
+            eapply All2_app => //. repeat constructor; auto. }
+          { move => [mfix1 [args1 [narg [fn' [[[[Hunf Hpre] Hpre']] a]]]]] eq.
+            subst M1.
+            rewrite /unfold_fix in Hunf.
+            red in Hpre.
+            case Heq: (nth_error mfix1 idx) Hunf => [d'|] //.
+            destruct (isLambda (dbody d')) eqn:isl => //. move => [=] Harg Hfn'.
+            subst fn' narg.
+            eapply All2_nth_error_Some_right in Heq; eauto.
+            destruct Heq as [d'' [nth' Hd'']]. rewrite nth' in e; noconf e.
+            move => redo.
+            rewrite map_app -mkApps_nested.
+            apply (pred_mkApps _ _ _ _ _ [N1] _).
+            case: Hd'' => reddd' [Hdd' deq].
+            noconf deq. simpl in H. noconf H. rewrite -H0 in Hpre'.
+            move: Hpre'; rewrite /is_constructor.
+            rewrite (All2_length _ _ a) in rargl.
+            rewrite rargl. rewrite (proj2 (nth_error_None _ _)). lia. discriminate.
+            repeat constructor; auto. }
+
+        ** (* None reduce *)
+          simpl. rewrite map_app.
+          rewrite -mkApps_nested => redo.
+          apply (pred_mkApps _ _ _ _ _ [N1] _). auto.
+          repeat constructor; auto.
+    + case le: (lambda_app_discr (tApp M0 N0)).
+      simpl in le'.
+      destruct M0; try discriminate.
+      (* Beta at top *)
+      depelim X. solve_discr.
+      depelim X0... econstructor; eauto.
+      discriminate.
+      rewrite rho_tApp_discr => //.
+      now apply: negbT. now apply: negbT.
+      constructor; auto.
+
+  - simpl. eapply pred_zeta; eauto.
+    now simpl in X4; rewrite app_context_nil_l in X4.
+
+  - (* Case reduction *)
+    red in X3.
+    destruct ind. destruct (decompose_app c0) eqn:Heq. simpl.
+    destruct (construct_cofix_discr t) eqn:Heq'; rewrite Heq.
+    destruct t; noconf Heq'.
+    + (* Iota *)
+      apply decompose_app_inv in Heq.
+      subst c0. simpl.
+      rewrite rho_mkApps; auto.
+      rewrite decompose_app_mkApps; auto.
+      simpl. rewrite rho_mkApps in X2; auto.
+      change eq_inductive with (@eqb inductive _).
+      destruct (eqb_spec i ind). subst ind.
+      eapply pred1_mkApps_tConstruct in X1 as [args' [? ?]]. subst c1.
+      eapply pred1_mkApps_refl_tConstruct in X2.
+      econstructor; eauto. pcuic.
+      eapply All2_sym, All2_map_left, All2_impl; eauto.
+      intros. hnf in X1. destruct X1. unfold on_Trel in *.
+      intuition pcuic.
+      econstructor; pcuic.
+      eapply All2_sym, All2_map_left, All2_impl; eauto.
+      intros. unfold on_Trel in *. intuition pcuic.
+
+    + (* CoFix *)
+      apply decompose_app_inv in Heq.
+      subst c0. simpl.
+      rewrite rho_mkApps; auto.
+      rewrite decompose_app_mkApps; auto.
+      simpl. rewrite rho_mkApps in X2; auto.
+      eapply pred1_mkApps_tCoFix_inv in X1 as [mfix' [idx' [[? ?] ?]]].
+      subst c1.
+      simpl in X2. eapply pred1_mkApps_tCoFix_refl_inv in X2.
+      intuition.
+      eapply All2_prop2_eq_split in a1. intuition.
+      unfold unfold_cofix. rewrite nth_error_map.
+      assert (All2 (on_Trel eq dname) mfix'
+                   (map_fix rho (rho_ctx Γ) (fold_fix_context rho (rho_ctx Γ) [] mfix) mfix)).
+      { eapply All2_impl; [eapply b0|]; pcuic. intros.
+        red in X1. now noconf X1. }
+      pose proof (All2_mix a1 X1).
+      eapply pred1_rho_fix_context_2 in X2; pcuic.
+      rewrite - fold_fix_context_rho_ctx in X2.
+      rewrite fix_context_map_fix in X2.
+      eapply rho_All_All2_local_env_inv in X2; pcuic.
+      rewrite - fold_fix_context_rho_ctx in a1.
+
+      destruct nth_error eqn:Heq. simpl.
+      * (* CoFix unfolding *)
+        pose proof Heq.
+        eapply All2_nth_error_Some in Heq; eauto. destruct Heq; intuition auto.
+
+        eapply pred_cofix_case with (map_fix rho (rho_ctx Γ) (rho_ctx_over (rho_ctx Γ)
+                                                                           (fix_context mfix)) mfix)
+                                    (rarg d); pcuic.
+
+        --- eapply All2_local_env_pred_fix_ctx; eauto.
+            eapply All2_prop2_eq_split in a. intuition auto.
+            eapply All2_local_env_sym.
+            pcuic.
+
+        --- eapply All2_mix; pcuic.
+            rewrite - fold_fix_context_rho_ctx in b1.
+            eapply All2_mix. eauto.
+            now rewrite - fold_fix_context_rho_ctx in b0.
+        --- unfold unfold_cofix.
+            rewrite nth_error_map.
+            rewrite H. simpl. f_equal. f_equal.
+            unfold map_fix.
+            rewrite fold_fix_context_rho_ctx. auto.
+        --- apply All2_sym. eapply All2_map_left. eapply All2_impl; eauto.
+            unfold on_Trel in *.
+            intros. intuition pcuic.
+
+      * eapply pred_case; eauto.
+        eapply pred_mkApps. constructor. pcuic.
+        --- rewrite - fold_fix_context_rho_ctx.
+            eapply All2_local_env_pred_fix_ctx.
+            eapply All2_prop2_eq_split in a. intuition auto.
+            eapply All2_local_env_sym.
+            pcuic.
+
+        --- eapply All2_mix; pcuic.
+            rewrite - fold_fix_context_rho_ctx in b1.
+            now rewrite - fold_fix_context_rho_ctx.
+            eapply All2_mix; pcuic.
+        --- pcuic.
+        --- eapply All2_sym, All2_map_left, All2_impl; eauto.
+            unfold on_Trel in *.
+            intros. intuition pcuic.
+
+    + apply decompose_app_inv in Heq. subst c0.
+      assert (All2 (on_Trel_eq (pred1 Σ Γ' (rho_ctx Γ)) snd fst) brs1
+                   (map (λ x : nat * term, (fst x, rho (rho_ctx Γ) (snd x))) brs0)).
+      { eapply All2_sym, All2_map_left, All2_impl; eauto.
+        unfold on_Trel in *.
+        intros. intuition pcuic. }
+      destruct t; try discriminate; simpl; pcuic.
+
+  - (* Proj *)
+    simpl.
+    destruct p as [[ind pars] arg].
+    destruct decompose_app eqn:Heq.
+    destruct (view_construct_cofix t).
+    + apply decompose_app_inv in Heq.
+      subst c. simpl.
+      rewrite rho_mkApps; auto.
+      rewrite decompose_app_mkApps; auto.
+      simpl. rewrite rho_mkApps in X0; auto.
+      simpl in X0.
+      pose proof (pred1_pred1_ctx _ X0).
+      eapply pred1_mkApps_tConstruct in X as [args' [? ?]]; subst.
+      eapply pred1_mkApps_refl_tConstruct in X0.
+      destruct nth_error eqn:Heq.
+      change eq_inductive with (@eqb inductive _).
+      destruct (eqb_spec ind c0); subst.
+      econstructor; eauto.
+      eapply pred_proj_congr, pred_mkApps; auto with pcuic. constructor; auto.
+      eapply pred_mkApps; auto.
+      econstructor; eauto.
+
+    + apply decompose_app_inv in Heq.
+      subst c. simpl.
+      rewrite rho_mkApps; auto.
+      rewrite decompose_app_mkApps; auto.
+      simpl. rewrite rho_mkApps in X0; auto. simpl in X0.
+      eapply pred1_mkApps_tCoFix_inv in X as [mfix' [idx' [[? ?] ?]]].
+      subst c'.
+      simpl in a.
+      pose proof X0.
+      eapply pred1_mkApps_tCoFix_refl_inv in X0.
+      destruct X0.
+      unfold unfold_cofix. rewrite nth_error_map.
+      eapply All2_prop2_eq_split in a1. intuition auto.
+      assert (All2 (on_Trel eq dname) mfix'
+                   (map_fix rho (rho_ctx Γ) (fold_fix_context rho (rho_ctx Γ) [] mfix) mfix)).
+      { eapply All2_impl; [eapply b|]; pcuic. intros.
+        red in X0. now noconf X0. }
+      pose proof (All2_mix a1 X0) as X2.
+      eapply pred1_rho_fix_context_2 in X2; pcuic.
+      rewrite - fold_fix_context_rho_ctx in X2.
+      rewrite fix_context_map_fix in X2.
+      eapply rho_All_All2_local_env_inv in X2; pcuic.
+      rewrite - fold_fix_context_rho_ctx in a1.
+      intuition auto.
+      destruct nth_error eqn:Heq. simpl.
+      (* Proj cofix *)
+      * (* CoFix unfolding *)
+        pose proof Heq.
+        eapply All2_nth_error_Some in Heq; eauto. destruct Heq; intuition auto.
+
+        eapply pred_cofix_proj with (map_fix rho (rho_ctx Γ) (rho_ctx_over (rho_ctx Γ)
+                                                                           (fix_context mfix)) mfix)
+                                    (rarg d); pcuic.
+
+        --- eapply All2_local_env_pred_fix_ctx; eauto.
+            eapply All2_prop2_eq_split in a. intuition auto.
+            eapply All2_local_env_sym.
+            pcuic.
+
+        --- eapply All2_mix; pcuic.
+            rewrite - fold_fix_context_rho_ctx in b0.
+            eapply All2_mix. eauto.
+            now rewrite - fold_fix_context_rho_ctx in b.
+        --- unfold unfold_cofix.
+            rewrite nth_error_map.
+            rewrite H. simpl. f_equal. f_equal.
+            unfold map_fix.
+            rewrite fold_fix_context_rho_ctx. auto.
+
+      * eapply pred_proj_congr; eauto.
+
+    + eapply decompose_app_inv in Heq. subst c.
+      destruct t; noconf d; econstructor; eauto.
+
+  - simpl.
+    rewrite - fold_fix_context_rho_ctx.
+    constructor; eauto.
+    now eapply All2_local_env_pred_fix_ctx. red. red in X3.
+    eapply All2_sym, All2_map_left, All2_impl; eauto.
+    simpl. unfold on_Trel; intuition pcuic.
+    rewrite rho_ctx_app in b. now rewrite fix_context_map_fix.
+
+  - simpl.
+    rewrite - fold_fix_context_rho_ctx.
+    constructor; eauto.
+    now eapply All2_local_env_pred_fix_ctx. red. red in X3.
+    eapply All2_sym, All2_map_left, All2_impl; eauto.
+    simpl. unfold on_Trel; intuition pcuic.
+    rewrite rho_ctx_app in b. now rewrite fix_context_map_fix.
+
+  - simpl; econstructor; eauto. simpl in X2. now rewrite !app_context_nil_l in X2.
+  - simpl in *. constructor. eauto. eapply All2_sym, All2_map_left, All2_impl. eauto.
+    intros. simpl in X. intuition.
+  - destruct t; noconf H; simpl; constructor; eauto.
+Qed.
+
 
   
